Tactic3.v
@@ -14,6 +14,8 @@ Arguments Id [C] _.
 Arguments Var [C X Y] _.
 Arguments Comp [C X Y Z] _ _.
 
+Hint Constructors exp.
+
 Fixpoint expDenote {C : Cat} {X Y : Ob C} (e : exp X Y)
     : Hom X Y :=
 match e with
@@ -21,6 +23,31 @@ match e with
     | Var f => f
     | Comp e1 e2 => expDenote e1 .> expDenote e2
 end.
+
+Fixpoint simplify {C : Cat} {X Y : Ob C} (e : exp X Y) {struct e} : exp X Y.
+Proof.
+  destruct e.
+    exact (Id _).
+    exact (Var h). destruct (simplify _ _ _ e1) as [| ? ? f1 | ? ? ? e11 e12]; clear e1.
+      exact (simplify _ _ _ e2).
+      destruct (simplify _ _ _ e2) as [| ? ? f2 | ? ? ? e21 e22]; clear e2.
+        exact (Var f1).
+        exact (Comp (Var f1) (Var f2)).
+        exact (Comp (Var f1) (Comp e21 e22)).
+      destruct (simplify _ _ _ e2) as [| ? ? f2 | ? ? ? e21 e22]; clear e2.
+        exact (Comp e11 e12).
+        exact (Comp (Comp e11 e12) (Var f2)).
+        exact (Comp (Comp e11 e12) (Comp e21 e22)).
+Defined.
+
+Theorem simplify_correct :
+  forall (C : Cat) (X Y : Ob C) (e : exp X Y),
+    expDenote (simplify e) == expDenote e.
+Proof.
+  induction e; simpl; try reflexivity.
+    destruct (simplify e1); destruct (simplify e2); simpl in *;
+    try rewrite <- IHe1; try rewrite <- IHe2; cat.
+Qed.
 
 Class PackedHom (C : Cat) : Type := mk
 {
@@ -47,17 +74,49 @@ end.
 Inductive wf {C : Cat} : list (PackedHom C) -> Prop :=
     | wf_nil : wf []
     | wf_singl : forall f : PackedHom C, wf [f]
-    | wf_cons : forall l1 l2 : list (PackedHom C),
+    | wf_app : forall l1 l2 : list (PackedHom C),
         wf l1 -> wf l2 -> wf (l1 ++ l2).
 
 Hint Constructors wf.
 
 Theorem flatten_wf :
-  forall (C : Cat) (X Y : Ob C) (e : exp X Y),
-    wf (flatten e).
+  forall (C : Cat) (X Y : Ob C) (e : exp X Y), wf (flatten e).
 Proof.
   induction e; simpl; auto.
 Qed.
+
+Inductive wf' {C : Cat} : list (PackedHom C) -> Prop :=
+    | wf'_nil : wf' []
+    | wf'_singl : forall f : PackedHom C, wf' [f]
+    | wf'_cons : forall (X : Ob C) (f g : PackedHom C)
+        (l : list (PackedHom C)),
+          cod f = dom g -> wf' (g :: l) -> wf' (f :: g :: l).
+
+Hint Constructors wf'.
+
+Lemma wf'_cod :
+  forall (C : Cat) (X Y : Ob C) (e : exp X Y) (h : PackedHom C)
+  (t : list (PackedHom C)),
+    flatten e = h :: t -> dom h = X.
+Proof.
+  induction e; inversion 1; cbn in *.
+    auto.
+    destruct e1; cbn in *; eauto.
+    destruct (flatten e2).
+      eapply IHe1. 
+Restart.
+  intros C X Y e. induction (flatten e) as [| h' t'].
+    inversion 1.
+Abort.
+
+Theorem flatten_wf' :
+  forall (C : Cat) (X Y : Ob C) (e : exp X Y), wf' (flatten e).
+Proof.
+  induction e; cbn; auto.
+    induction (flatten e1); cbn; auto. destruct l.
+      Focus 2. cbn. inversion IHe1; subst; auto.
+      destruct (flatten e2); cbn in *; auto. constructor; auto.
+Abort.
 
 Theorem flatten_cons :
   forall (C : Cat) (h : PackedHom C) (t : list (PackedHom C)),
@@ -65,7 +124,8 @@ Theorem flatten_cons :
 Proof.
   induction t; simpl; auto.
     inversion 1. subst.
-    
+Abort.
+
 Theorem flatten_wf_inv :
   forall (C : Cat) (l l1 l2 : list (PackedHom C)),
     wf l -> l = l1 ++ l2 -> wf l1 /\ wf l2.
@@ -76,15 +136,11 @@ Proof.
       rewrite app_comm_cons in H0. inversion H0; subst.
       rewrite app_comm_cons in H. inversion H; subst. Focus 2.
       inversion H.
-      change (h :: t) with ([h] ++ t) in H. inversion H; subst.
-        inversion H0. destruct l1; simpl in *; inversion H0; auto.
-        
+Abort.
 
-Fixpoint expDenote
-
-Lemma expDenoteHL_comp_app :
+(*Lemma expDenoteHL_comp_app :
   forall (C : Cat) (X Y Z : Ob C) (l1 : HomList X Y) (l2 : HomList Y Z),
-    expDenoteHL l1 .> expDenoteHL l2 == expDenoteHL (l1 +++ l2).
+    expDenoteHL l1 .> expDenoteHL l2 == expDenoteHL (l1 ++ l2).
 Proof.
   induction l1; simpl; intros.
     rewrite id_left. reflexivity.
@@ -105,9 +161,7 @@ Theorem cat_reflect :
     expDenoteHL (flatten (simplify e2)) ->
       expDenote e1 == expDenote e2.
 Proof.
-  intros.
-  do 2 rewrite flatten_correct in H.
-  do 2 rewrite simplify_correct in H.
+  intros. rewrite !flatten_correct, !simplify_correct in H.
   assumption.
 Qed.
 
@@ -216,4 +270,4 @@ Proof.
   induction e; simpl; try reflexivity.
     destruct (simplify' e1); destruct (simplify' e2); simpl in *;
     try rewrite <- IHe1; try rewrite <- IHe2; cat.
-Qed.
+Qed.*)
